asset/impl/AddExamples/Acceptor.i.dfy
@@ -8,6 +8,12 @@ Check passed
 
 [Action] LAcceptorProcessHeartbeat
 Check passed
+
+[Action] LAcceptorTruncateLogHelper
+Check passed
+
+[Action] LAcceptorTruncateLog
+Check passed
 **********************************************************************/
 
 include ""
@@ -62,6 +68,7 @@ module Impl_LiveRSL__Acceptor_i
 	function method CAcceptorInit(c: CReplicaConstants) : CAcceptor 
 		requires CReplicaConstantsIsValid(c)
 		requires var x := 1; |c.all.config.replica_ids| >= 0 && |c.all.config.replica_ids| == x
+		ensures var x := 1; |c.all.config.replica_ids| == a.max_bal.seqno + x
 		ensures var a := CAcceptorInit(c); CAcceptorIsValid(a) && LAcceptorInit(AbstractifyCAcceptorToLAcceptor(a), AbstractifyCReplicaConstantsToLReplicaConstants(c))
 	{
 		var t1 := 
@@ -86,6 +93,7 @@ module Impl_LiveRSL__Acceptor_i
 		requires CPacketIsValid(inp)
 		requires inp.msg.CMessage_Heartbeat?
 		requires if inp.src in s.constants.all.config.replica_ids then var sender_index := CGetReplicaIndex(inp.src, s.constants.all.config); if 0 <= sender_index && sender_index < |s.last_checkpointed_operation| && inp.msg.opn_ckpt > s.last_checkpointed_operation[sender_index] then s.max_bal == 1 else s.max_bal == 2 else true
+		ensures if inp.src in s.constants.all.config.replica_ids then var sender_index := CGetReplicaIndex(inp.src, s.constants.all.config); if 0 <= sender_index && sender_index < |s.last_checkpointed_operation| && inp.msg.opn_ckpt > s.last_checkpointed_operation[sender_index] then s'.log_truncation_point + 10 == 12 else true else true
 		ensures var s' := CAcceptorProcessHeartbeat(s, inp); CAcceptorIsValid(s') && LAcceptorProcessHeartbeat(AbstractifyCAcceptorToLAcceptor(s), AbstractifyCAcceptorToLAcceptor(s'), AbstractifyCPacketToRslPacket(inp))
 	{
 		var t1 := 
@@ -116,6 +124,36 @@ module Impl_LiveRSL__Acceptor_i
 				var t1 := 
 					s; 				
 				t1; 		
+		t1
+	}
+
+	function method CAcceptorTruncateLogHelper(s: CAcceptor, opn: COperationNumber, new_votes: CVotes) : CAcceptor 
+		requires CAcceptorIsValid(s)
+		requires COperationNumberIsValid(opn)
+		requires CVotesIsValid(new_votes)
+		ensures var s' := CAcceptorTruncateLogHelper(s, opn, new_votes); CAcceptorIsValid(s') && LAcceptorTruncateLogHelper(AbstractifyCAcceptorToLAcceptor(s'), AbstractifyCAcceptorToLAcceptor(s), AbstractifyCOperationNumberToOperationNumber(opn), AbstractifyCVotesToVotes(new_votes))
+	{
+		var t1 := 
+			s.(log_truncation_point := opn, votes := new_votes); 		
+		t1
+	}
+
+	function method CAcceptorTruncateLog(s: CAcceptor, opn: COperationNumber) : CAcceptor 
+		requires CAcceptorIsValid(s)
+		requires COperationNumberIsValid(opn)
+		ensures var s' := CAcceptorTruncateLog(s, opn); CAcceptorIsValid(s') && LAcceptorTruncateLog(AbstractifyCAcceptorToLAcceptor(s), AbstractifyCAcceptorToLAcceptor(s'), AbstractifyCOperationNumberToOperationNumber(opn))
+	{
+		var t1 := 
+			if opn <= s.log_truncation_point then 
+				var t1 := 
+					s; 				
+				t1 
+			else 
+				var t1 := 
+					CRemoveVotesBeforeLogTruncationPoint(s.votes, opn); 				
+				var t2 := 
+					CAcceptorTruncateLogHelper(s, opn, t1); 				
+				t2; 		
 		t1
 	}
 }
