cnt_lines.sh
@@ -1,0 +1,1 @@
+find lib test -type f \( -name "*.ml" -o -name "*.mll" -o -name "*.mly" \) -exec wc -l {} +
